theories/MorphismsFacts.v
@@ -177,18 +177,81 @@ Proof.
     eapply (CIH' (go x2) (go x3)); eauto.
   - rewrite !bind_unfold. fold_bind.
     genobs t ot. clear Heqot t.
-    destruct ot; simpl; eauto 10 using gres2.
+    destruct ot; simpl; eauto 10. 
     pfold. eapply euttF'_mon; eauto using interp_inv_main_step; intros.
     eapply upaco2_mon; eauto. intros.
     eapply (CIH' (go x2) (go x3)); eauto.
 Qed.
 
+
+Lemma unfold_interp_state : forall {E F S R} (h : E ~> Monads.stateT S (itree F)) t s,
+    observe (interp_state h _ t s) =
+    observe (interp_state_match h (interp_state h R) t s).
+Proof.
+  intros E F S R h t s.
+  econstructor.
+Qed.  
+
+
+Instance eq_itree_interp_state {E F S R} (h : E ~> Monads.stateT S (itree F)) :
+  Proper (@eq_itree E R ==> @eq S ==>
+          @eq_itree F (S * R)) (interp_state h _).
+Proof.
+  repeat intro. pupto2_init. revert_until R.
+  pcofix CIH. intros h x y H0 x2 y0 H1. 
+  rewrite itree_eta, (itree_eta (interp_state h _ y y0)), !unfold_interp_state.
+  unfold interp_state_match.
+  punfold H0; red in H0.
+  genobs x ox; destruct ox; simpobs; dependent destruction H0; simpobs; pclearbot.
+  - pupto2_final. pfold. red. cbn. subst. eauto.
+  - pupto2_final. pfold. red. cbn. subst. eauto.
+  - pfold. econstructor. pupto2 (eq_itree_clo_bind F (S * R)).
+    constructor.
+    + subst. reflexivity.
+    + intros; pupto2_final; right; eauto.
+Qed.
+
+
+Lemma interp_state_ret {E F : Type -> Type} {R S : Type}
+      (f : forall T, E T -> S -> itree F (S * T)%type)
+      (s : S) (r : R) :
+  (interp_state f _ (Ret r) s) ≅ (Ret (s, r)).
+Proof.
+  rewrite itree_eta. reflexivity.
+Qed.
+
+
+Lemma interp_state_vis : forall {E F:Type -> Type} {S T U : Type} (s:S) e k
+                           (h : E ~> Monads.stateT S (itree F)),
+    interp_state h U (Vis e k) s ≅ Tau (ITree.bind (h T e s) (fun sx => interp_state h _ (k (snd sx)) (fst sx))).
+Proof.
+  intros E F S T U s e k h.
+  rewrite itree_eta.
+  reflexivity.
+Qed.
+
+Lemma interp_state_tau : forall {E F:Type -> Type} S {T : Type} (t:itree E T) (s:S)
+                           (h : E ~> Monads.stateT S (itree F)),
+    interp_state h _ (Tau t) s ≅ Tau (interp_state h _ t s).
+Proof.
+  intros E F S T t s h. 
+  rewrite itree_eta. reflexivity.
+Qed.
+
 Lemma interp_state_liftE {E F : Type -> Type} {R S : Type}
       (f : forall T, E T -> S -> itree F (S * T)%type)
       (s : S) (e : E R) :
-  (interp_state f _ (ITree.liftE e) s) ≅ (f _ e s).
+  (interp_state f _ (ITree.liftE e) s) ~~ (f _ e s).
 Proof.
-Admitted.
+  unfold ITree.liftE. rewrite interp_state_vis.  
+  rewrite tau_eutt.
+  assert (pointwise_relation _ eq_itree (fun sx : S * R => interp_state f R (Ret (snd sx)) (fst sx)) (fun sx => Ret sx)).
+  { intros sx. destruct sx. simpl.
+    rewrite itree_eta. cbn. reflexivity. }
+  rewrite H.
+  cbn. rewrite bind_ret.
+  reflexivity.
+Qed.  
 
 Lemma interp_state_bind {E F : Type -> Type} {A B S : Type}
       (f : forall T, E T -> S -> itree F (S * T)%type)
@@ -198,11 +261,20 @@ Lemma interp_state_bind {E F : Type -> Type} {A B S : Type}
     ≅
   (interp_state f _ t s >>= fun st => interp_state f _ (k (snd st)) (fst st)).
 Proof.
-Admitted.
+  pupto2_init.
+  revert A t k s.
+  pcofix CIH.
+  intros A t k s.
+  rewrite (itree_eta t).
+  destruct (observe t).
+  - cbn. rewrite interp_state_ret. rewrite !ret_bind. simpl.
+    pupto2_final. apply eq_itree_refl.
+  - cbn. rewrite interp_state_tau, !tau_bind, interp_state_tau.
+    pupto2_final. pfold. econstructor. right. apply CIH.
+  - cbn. rewrite interp_state_vis, tau_bind, vis_bind, bind_bind, interp_state_vis.
+    pfold. red. constructor.
+    pupto2 (eq_itree_clo_bind F (S * B)). econstructor.
+    + reflexivity.
+    + intros. specialize (CIH _ (k0 (snd v)) k (fst v)). auto.
+Qed.      
 
-Lemma interp_state_ret {E F : Type -> Type} {R S : Type}
-      (f : forall T, E T -> S -> itree F (S * T)%type)
-      (s : S) (r : R) :
-  (interp_state f _ (Ret r) s) ≅ (Ret (s, r)).
-Proof.
-Admitted.
